[ZOJ_3925](http://acm.zju.edu.cn/onlinejudge/showProblem.do?problemCode=3925)


m[i..j]表示，石头是[i..j]时的最优解，则

```
当i==j时，
    m[i..j] = m[i..i] = d[i]
```
```
当Count(i..j)==2时，
    m[i..j] = m[i..i] = d[i] + d[j]
```
```
当Count(i..j)>=3时，
    定义k，i <= k <=j 
    k==i时，
        m[i..j] = m[i..i] + m[i+1..j]
    k==j时，
        m[i..j] = m[j..j] + m[i..j-1]
    i+1<=k<=j-1时
        m[i..j] = min { k | max{ m[i..k-1] + m[k..k], m[k..k] + m[k+1..j] } }
    所以，
        取 i+1<=k<=j-1时
        m[i..j] = min { 
                    min { k | max{ m[i..k-1] + m[k..k], m[k..k] + m[k+1..j] } },
                    m[i..i] + m[i+1..j],
                    m[j..j] + m[i..j-1]
                  }
        展开min看看：
            m[i..j] = min { 
                                                m[i..i] + m[i+1..j],
                    
                    max{ m[i..i] + m[i+1..i+1], m[i+1..i+1] + m[i+2..j] },   // k=i+1
                    max{ m[i..i+1] + m[i+2..i+2], m[i+2..i+2] + m[i+3..j] }, //k=i+2
                    ...
                    max{ m[i..k-1] + m[k..k], m[k..k] + m[k+1..j] }
                    ...
                    max{ m[i..j-2] + m[j-1..j-1], m[j-1..j-1] + m[j..j] },    //k=j-1
                    
                        m[i..j-1] + m[j..j] 
                  }
```
起始公式，
当Count(i..j)==3时，
        j = i+2
        m[i..j] = min { 
            max{ m[i..i] + m[i+1..i+1], m[i+1..i+1] + m[i+2..i+2] } //k=i+1
            m[i..i] + m[i+1..i+1] + m[i+2..i+2]
            m[i..i] + m[i+1..i+1] + m[i+2..i+2]
        }
        所以
        m[i..j] = min { 
            max{ m[i..i] + m[i+1..i+1], m[i+1..i+1] + m[i+2..j] }, // k=i+1
            max{ m[i..i+1] + m[i+2..i+2], m[i+2..i+2] + m[i+3..j] }, //k=i+2
            ...
            max{ m[i..k-1] + m[k..k], m[k..k] + m[k+1..j] }
            ...
            max{ m[i..j-2] + m[j-1..j-1], m[j-1..j-1] + m[j..j] },//k=j-1
        } <= m[i..i] + m[i+1..j], m[j..j] + m[i..j-1]
        成立。
假设Count(i..j)时，公式成立，即
        
        m[i..j] = min { 
            max{ m[i..i] + m[i+1..i+1], m[i+1..i+1] + m[i+2..j] }, // k=i+1
            max{ m[i..i+1] + m[i+2..i+2], m[i+2..i+2] + m[i+3..j] }, //k=i+2
            ...
            max{ m[i..k-1] + m[k..k], m[k..k] + m[k+1..j] }
            ...
            max{ m[i..j-2] + m[j-1..j-1], m[j-1..j-1] + m[j..j] },//k=j-1
        } <= m[i..i] + m[i+1..j], m[i..j-1] + m[j..j]

那么Count(i..j+1)时，
    不等式左边：
        m[i..j+1] = min { 
            max{ m[i..i] + m[i+1..i+1], m[i+1..i+1] + m[i+2..j+1] }, // k=i+1
            max{ m[i..i+1] + m[i+2..i+2], m[i+2..i+2] + m[i+3..j+1] }, //k=i+2
            ...
            max{ m[i..k-1] + m[k..k], m[k..k] + m[k+1..j+1] }
            ...
            max{ m[i..j-2] + m[j-1..j-1], m[j-1..j-1] + m[j..j] },//k=j-1
            
            max{ m[i..j-1] + m[j..j], m[j..j] + m[j+1..j+1] },//k=j
        } 
        
        
        m[i..i] + m[i+1..j+1] <= m[i..i] + m[i+1..j] + m[j+1..j+1], 
        m[i..j] + m[j+1..j+1] <= m[i..j-1] + m[j..j] + m[j+1..j+1]
    
因为当n=3时,k一定取2。

一般性公式：
当Count(i..j)>=3时，
1<=i<=j-2<=n, i+1<=k<=j-1
    min { k | max{ m[i..k-1] + m[k..k], m[k..k] + m[k+1..j] } <= m[i..i] + m[i+1..j]
    min { k | max{ m[i..k-1] + m[k..k], m[k..k] + m[k+1..j] } <= m[j..j] + m[i..j-1]